README.md
@@ -6,6 +6,8 @@ Paper at: https://arxiv.org/abs/1802.01336
 The paper corresponds to the initial commit 8d336cd, which uses the version
 of auto2 (https://github.com/bzhan/auto2) at commit 167808b.
 
+The current commit corresponds to commit d582abd in auto2.
+
 ### Abstract:
 
 We present a framework in Isabelle for verifying asymptotic time
